---
problem: 3.1.2.13
layout: problem
textbook: ctfs
---

> Consider the functions $\phi$ and $\psi$ above.
>
> _a)_ Show that for any
> $\delta:\Sigma\times S\to S$, the map $\psi(\delta): \text{List}(\Sigma)\times
> S \to S$ constitutes an action.

For a finite state machine $\text{FSM} := (\Sigma, S, \delta, s_0, F)$:
 - $\Sigma$ is a finite, non-empty set of symbols (the _input alphabet_) of a
   deterministic finite state machine.
 - $S$ is a finite, non empty set of _states_ in that finite state machine,
 - $\delta:\Sigma\times S\to S$ is the _state-transition function_ of that
   machine.
 - $ A = \\{ \epsilon: \text{List}(\Sigma) \times S \to S \mid \epsilon \text{
   constitutes an action} \\} $ is the set of $\Sigma$-actions on $S$.
 - $ \phi: A\stackrel\cong\to S^{\Sigma\times S}$, which isomorphically
   maps between $A$ and $S^{\Sigma\times S}$.
 - $ \psi: S^{\Sigma\times S} \to A$ is the inverse of $\phi$, defined over a
   list $L=[\epsilon_1,...\epsilon_n]$ and $L' = [\epsilon_1,...\epsilon_{n-1}]$
   as $\psi(f)(\lbrack\ \rbrack,s) = s$ and $\psi(f)(L,s) = \psi(f)(L',
   f(\epsilon_n, s))$.
 - $ \psi(\delta): \text{List}(\Sigma)\times S\to S$, the inverse of $\phi$ as
   applied to a single element $\delta$, which _might_ be seen as an action of
   $\text{List}(\Sigma)$ on $S$, or a $\text{List}(\Sigma)$-action on $S$.

From the definition of $\psi$, we can see:

$$ 
\begin{align}
\psi(f)(L,s) \mid_{L = \lbrack\ \rbrack} 
&= \psi(f)(\lbrack\ \rbrack, s) \\
&= s \\
e\cdot s &= s &&(e = \lbrack\ \rbrack)
\end{align}
$$

and (also from the definition of $\psi$),

$$
\begin{align}
\psi(f)(m\pp n,s) 
&= \psi(f)(\lbrack m_1, ...m_i, n_1, ...n_j \rbrack, s) \\
&= \psi(f)(\lbrack m_1, ...m_i, n_1, ...n_{j-1} \rbrack, f(n_j, s)) \\
&= ... \\
&= \psi(f)(\lbrack m_1, ...m_i \rbrack, f(n_1, f(... f(n_j, s)))) \\
\psi(f)(m\pp n, s) &= \psi(f)(m, \psi(f)(n,s)) \\
(m\star n) \cdot s &= m\cdot(n\cdot s)
\end{align}
$$

Thus $\psi(f)$ is an action of $\text{List}(\Sigma)$ on $S$.

> _b)_ Show that $\phi$ and $\psi$ are mutually inverse functions (i.e.
> $\phi\circ\psi = \id_{\text{Hom}(\Sigma\times S, S)}$ and $\psi\circ\phi =
> \id_A$.)

For a function $f:\Sigma\times S\to S$, $(\phi\circ\psi)(f) = \phi(\psi(f)) = 
